Rework compute_labels more seriously
Remove lab_insert; change the rest of the algorithm in the hope that it
will be faster. Also, start updating the proofs because it's not so
clear the new version is correct. There are two cheats (one fairly big)
in the proof.

compiler/backend/lab_to_targetScript.sml
@@ -43,34 +43,14 @@ val enc_sec_list_def = Define `
 
 (* compute labels *)
 
-val asm_line_labs_def = Define `
-  (asm_line_labs pos [] acc = (acc,pos)) /\
-  (asm_line_labs pos ((Label k1 k2 l)::xs) acc =
-     asm_line_labs (pos+l) xs (union acc (insert k2 (pos+l) LN))) /\
-  (asm_line_labs pos ((Asm _ _ l)::xs) acc =
-     asm_line_labs (pos+l) xs acc) /\
-  (asm_line_labs pos ((LabAsm _ _ _ l)::xs) acc =
-     asm_line_labs (pos+l) xs acc)`
-
-val sec_labs_def = Define `
-  sec_labs pos lines =
-    asm_line_labs pos lines (insert 0 pos LN)`;
-
-val lab_insert_def = Define `
-  lab_insert l1 l2 pos labs =
-    insert l1 (insert l2 pos
-      (case lookup l1 labs of
-       | NONE => LN
-       | SOME t => t)) labs`
-
 val section_labels_def = Define `
-  (section_labels pos [] labs = labs) /\
-  (section_labels pos (Label l1 l2 len :: xs) labs =
+  (section_labels pos [] labs = (pos,labs)) /\
+  (section_labels pos (Label _ l2 len :: xs) labs =
      (*Ignore 0 labels*)
      if l2 = 0 then
        section_labels (pos+len) xs labs
      else
-       section_labels (pos+len) xs (lab_insert l1 l2 (pos+len) labs)) /\
+       section_labels (pos+len) xs ((l2,pos+len)::labs)) /\
   (section_labels pos (Asm _ _ len :: xs) labs =
      section_labels (pos+len) xs labs) /\
   (section_labels pos (LabAsm _ _ _ len :: xs) labs =
@@ -79,9 +59,9 @@ val section_labels_def = Define `
 val compute_labels_alt_def = Define `
   (compute_labels_alt pos [] labs = labs) /\
   (compute_labels_alt pos (Section k lines::rest) labs =
-    let new_pos = sec_length lines 0 in
-    compute_labels_alt (pos+new_pos) rest
-      (lab_insert k 0 pos (section_labels pos lines labs)))`
+    let (new_pos,sec_labs) = section_labels pos lines [] in
+    compute_labels_alt new_pos rest
+      (insert k (fromAList ((0,pos)::sec_labs)) labs))`
 
 (* update code, but not label lengths *)
 
@@ -222,41 +202,6 @@ val pad_code_def = Define `
 (pad_code nop [] = []) /\
 (pad_code nop ((Section n xs)::ys) =
   Section n (pad_section nop xs []) :: pad_code nop ys)`
-
-(* some final checks on the result *)
-
-val loc_to_pc_comp_def = Define `
-  loc_to_pc_comp n1 n2 [] = NONE /\
-  loc_to_pc_comp n1 n2 (Section k xs::ys) =
-    if k = n1 ∧ n2 = 0 then SOME 0n
-    else
-      case xs of
-        [] => loc_to_pc_comp n1 n2 ys
-      | z::zs =>
-        case z of
-        | Label k1 k2 _ =>
-            if k1 = n1 /\ k2 = n2 /\ n2 <> 0 then SOME 0
-            else loc_to_pc_comp n1 n2 (Section k zs::ys)
-        | _ => case loc_to_pc_comp n1 n2 (Section k zs::ys) of
-                 NONE => NONE
-               | SOME pos => SOME (pos + 1)`
-
-val is_Label_def = Define `
-  (is_Label (Label _ _ _) = T) /\
-  (is_Label _ = F)`;
-val _ = export_rewrites["is_Label_def"];
-
-val check_lab_def = Define `
-  check_lab sec_list (l1,l2,pos) <=>
-    EVEN pos`
-
-val all_labels_def = Define `
-  all_labels labs =
-    FLAT (MAP (\(n,t). MAP (\x. (n, x)) (toAList t)) (toAList labs))`
-
-val sec_names_def = Define`
-  (sec_names [] = []) ∧
-  (sec_names ((Section k _)::xs) = k::sec_names xs)`
 
 (* top-level assembler function *)
 
